Update 06 11
- Apply step translate validated
- Benchmark updated
- Refactoring encoding

Pacman_TransformationCorrectness/PacmanP1.bpl
@@ -1,37 +1,11 @@
+
+
+
 procedure driver();
 requires $IsGoodHeap($srcHeap);
-requires (forall pac1,pac2: ref::
-	pac1 != null && read($srcHeap,pac1,alloc) && dtype(pac1) == pacman$Pacman
-&&	pac2 != null && read($srcHeap,pac2,alloc) && dtype(pac2) == pacman$Pacman
-==>
-	pac1 == pac2
-);
-requires (forall r1,r2: ref::
-	r1 != null && read($srcHeap,r1,alloc) && dtype(r1) == pacman$Record
-&&	r2 != null && read($srcHeap,r2,alloc) && dtype(r2) == pacman$Record
-==>
-	r1 ==r2
-);
-requires (forall<alpha> grid: ref :: 
-	grid != null && read($srcHeap,grid,alloc) && dtype(grid) == pacman$Grid
-	&& read($srcHeap,grid,pacman$Grid.hasGem)!=null && read($srcHeap,read($srcHeap,grid,pacman$Grid.hasGem),alloc)
-	==>
-	dtype(read($srcHeap,grid,pacman$Grid.hasGem)) == pacman$Gem
-);
-requires (forall<alpha> grid1, grid2: ref :: 
-	grid1 != null && read($srcHeap,grid1,alloc) && dtype(grid1) == pacman$Grid
-&&	grid2 != null && read($srcHeap,grid2,alloc) && dtype(grid2) == pacman$Grid
-	/* grid1 can equal to grid2 */
-	==>
-	reachable($srcHeap, grid1, grid2)
-);
-requires  !(forall<alpha> grid1, grid2: ref :: 
-	grid1 != null && read($srcHeap,grid1,alloc) && dtype(grid1) == pacman$Grid
-&&	grid2 != null && read($srcHeap,grid2,alloc) && dtype(grid2) == pacman$Grid
-==>  (read($srcHeap,grid1,pacman$Grid.hasPlayer) != null 
-	&& read($srcHeap,grid2,pacman$Grid.hasEnemy) != null)
-);
-modifies $srcHeap;
+requires $Well_form($srcHeap);
+requires lemma_col($srcHeap, col);
+modifies $srcHeap, col;
 ensures  (forall<alpha> grid1, grid2: ref :: 
 	grid1 != null && read($srcHeap,grid1,alloc) && dtype(grid1) == pacman$Grid
 &&	grid2 != null && read($srcHeap,grid2,alloc) && dtype(grid2) == pacman$Grid
@@ -44,7 +18,9 @@ ensures  (forall<alpha> grid1, grid2: ref ::
 		==>
 		reachable($srcHeap, grid1, grid2)
 	)	
-);
+); 
+ensures  $Well_form($srcHeap);
+ensures  lemma_col($srcHeap, col);
 
 
 
@@ -60,7 +36,11 @@ var grid1#0: ref;
 var grid2#0: ref;
 var act#0: ref;
 
-
+var s#4: ref;
+var rec#4: ref;
+var pac#4: ref;
+var grid1#4: ref;
+var act#4: ref;
 
 var s#5: ref;
 var rec#5: ref;
@@ -68,6 +48,12 @@ var ghost#5: ref;
 var grid1#5: ref;
 var grid2#5: ref;
 var act#5: ref;
+
+var s#8: ref;
+var rec#8: ref;
+var ghost#8: ref;
+var grid1#8: ref;
+var act#8: ref;
 
 var s#9: ref;
 var rec#9: ref;
@@ -107,38 +93,8 @@ var b#11: bool;
 
 
 while(true)
-  invariant (forall<alpha> grid: ref :: 
-	grid != null && read(old($srcHeap),grid,alloc) && dtype(grid) == pacman$Grid 
-	==>
-		read($srcHeap, grid, alloc) 
-  );
-  invariant  (forall<alpha> grid: ref, f: Field alpha :: 
-	grid != null && read(old($srcHeap),grid,alloc) && dtype(grid) == pacman$Grid 
-	<==> grid != null && read($srcHeap,grid,alloc) && dtype(grid) == pacman$Grid  
-  );
-  invariant  (forall<alpha> grid: ref, f: Field alpha :: 
-	grid != null && read(old($srcHeap),grid,alloc) && dtype(grid) == pacman$Grid ==>
-		(read($srcHeap, grid, f) == read(old($srcHeap), grid, f)
-		|| f==pacman$Grid.hasPlayer || f==pacman$Grid.hasEnemy || f==pacman$Grid.hasGem)
-  );
-  invariant (forall<alpha> grid1, grid2: ref :: 
-	grid1 != null && read($srcHeap,grid1,alloc) && dtype(grid1) == pacman$Grid
-&&	grid2 != null && read($srcHeap,grid2,alloc) && dtype(grid2) == pacman$Grid
-	/* grid1 can equal to grid2 */
-	==>
-	reachable($srcHeap, grid1, grid2));
-  invariant (forall pac1,pac2: ref::
-	pac1 != null && read($srcHeap,pac1,alloc) && dtype(pac1) == pacman$Pacman
-&&	pac2 != null && read($srcHeap,pac2,alloc) && dtype(pac2) == pacman$Pacman
-==>
-	pac1 == pac2
-); 
-  invariant   !(forall<alpha> grid1, grid2: ref :: 
-	grid1 != null && read($srcHeap,grid1,alloc) && dtype(grid1) == pacman$Grid
-&&	grid2 != null && read($srcHeap,grid2,alloc) && dtype(grid2) == pacman$Grid
-==> ( read($srcHeap,grid1,pacman$Grid.hasPlayer) != null 
-	&& read($srcHeap,grid2,pacman$Grid.hasEnemy) != null)
-);
+invariant $Well_form($srcHeap);
+invariant lemma_col($srcHeap, col);
 {
 
 	match_PlayerMoveLeft:	
@@ -149,17 +105,34 @@ while(true)
 	apply_PlayerMoveLeft:
 		if(todo!=Seq#Empty()){
 			// execute applier block start
-			s#0 := Seq#Index(todo,0);
-			rec#0 := Seq#Index(todo,1);
-			pac#0 := Seq#Index(todo,2);
-			grid2#0 := Seq#Index(todo,3);
-			grid1#0 := Seq#Index(todo,4);
-			act#0 := Seq#Index(todo,5);
-	
-			$srcHeap := update($srcHeap, s#0, pacman$GameState.STATE, 4);
-			$srcHeap := update($srcHeap, grid1#0, pacman$Grid.hasPlayer, null);
-			$srcHeap := update($srcHeap, grid2#0, pacman$Grid.hasPlayer, pac#0);
-			$srcHeap := update($srcHeap, act#0, alloc, false);
+			
+			call apply_PlayerMoveLeft(todo);
+				
+			// havoc act#0; as a alternative to dispose act#0
+			// act#0 := null;
+			
+			
+			// update finished, Heap should still be in a valid state.
+
+			// exists RHS
+			
+			// Termination Metric 
+
+			// restart
+			goto restart;
+		}else{
+			goto match_PlayerStay;
+		}
+
+	match_PlayerStay:	
+		havoc todo;
+		call todo := match_PlayerStay();
+		goto apply_PlayerStay;
+				
+	apply_PlayerStay:
+		if(todo!=Seq#Empty()){
+			// execute applier block start
+			call apply_PlayerStay(todo);
 			// havoc act#0; as a alternative to dispose act#0
 			// act#0 := null;
 			
@@ -186,21 +159,29 @@ while(true)
 	apply_GhostMoveLeft:
 		if(todo!=Seq#Empty()){
 			// execute applier block start
-			s#5 := Seq#Index(todo,0);
-			rec#5 := Seq#Index(todo,1);
-			ghost#5 := Seq#Index(todo,2);
-			grid2#5 := Seq#Index(todo,3);
-			grid1#5 := Seq#Index(todo,4);
-			act#5 := Seq#Index(todo,5);
+			call apply_GhostMoveLeft(todo);
+			// update finished, Heap should still be in a valid state.
 
-
+			// exists RHS
 			
+			// Termination Metric 
 
-			
-			$srcHeap := update($srcHeap, s#5, pacman$GameState.STATE, 5);
-			$srcHeap := update($srcHeap, grid1#5, pacman$Grid.hasEnemy, null);
-			$srcHeap := update($srcHeap, grid2#5, pacman$Grid.hasEnemy, ghost#5);
-			$srcHeap := update($srcHeap, act#5, alloc, false);
+			// restart
+			goto restart;
+		}else{
+			goto match_GhostStay;
+		}
+	
+	match_GhostStay:	
+		havoc todo;
+		call todo := match_GhostStay();
+		goto apply_GhostStay;
+
+				
+	apply_GhostStay:
+		if(todo!=Seq#Empty()){
+			// execute applier block start
+			call apply_GhostStay(todo);
 			
 			// update finished, Heap should still be in a valid state.
 
@@ -216,8 +197,7 @@ while(true)
 		}else{
 			goto match_Collect;
 		}
-	
-
+		
 	match_Collect:	
 		havoc todo;
 		call todo := match_Collect();
@@ -225,46 +205,15 @@ while(true)
 		
 	apply_Collect:
 		if(todo!=Seq#Empty()){
-			// execute applier block start
-			s#9 := Seq#Index(todo,0);
-			rec#9 := Seq#Index(todo,1);
-			pac#9 := Seq#Index(todo,2);
-			gem#9 := Seq#Index(todo,3);
-			grid#9 := Seq#Index(todo,4);
-
-
-			assert (forall<alpha> grid: ref :: 
-	grid != null && read(old($srcHeap),grid,alloc) && dtype(grid) == pacman$Grid 
-	==>
-		read($srcHeap, grid, alloc) 
-  );
-
-			
+		
 			// newRecord
 			havoc recordNew#9;
-			assume recordNew#9 != null && !read($srcHeap, recordNew#9, alloc) && dtype(recordNew#9) == 
-			pacman$Record;
-			$srcHeap := update($srcHeap, recordNew#9, alloc, true);
-			assume $IsGoodHeap($srcHeap);
+			assume recordNew#9 != null && !read($srcHeap, recordNew#9, alloc) && dtype(recordNew#9) == pacman$Record;
 			
-			// gameState.record = newRecord
-			$srcHeap := update($srcHeap, s#9, pacman$GameState.record, recordNew#9);
-			
-			// initialize newRecord
-			$srcHeap := update($srcHeap, recordNew#9, pacman$Record.FRAME, read($srcHeap, rec#9, pacman$Record.FRAME));
-			
-			$srcHeap := update($srcHeap, recordNew#9, pacman$Record.SCORE, read($srcHeap, rec#9, pacman$Record.SCORE)+100);
-			
+	
+			// execute applier block start
 
-			
-			// Grid.hasGem = null
-			$srcHeap := update($srcHeap, grid#9, pacman$Grid.hasGem, null);
-			
-			// gem.alloc = false
-			$srcHeap := update($srcHeap, gem#9, alloc, false);
-			
-			// rec.alloc = false
-			$srcHeap := update($srcHeap, rec#9, alloc, false);
+			call apply_Collect(todo, recordNew#9);
 			
 			// update finished, Heap should still be in a valid state.
 
@@ -288,23 +237,10 @@ while(true)
 	apply_Kill:
 		if(todo!=Seq#Empty()){
 			// execute applier block start
-			s#10 := Seq#Index(todo,0);
-			ghost#10 := Seq#Index(todo,1);
-			pac#10 := Seq#Index(todo,2);
-			grid#10 := Seq#Index(todo,3);
 
-
-			// Grid.hasPlayer = null
-			$srcHeap := update($srcHeap, grid#10, pacman$Grid.hasPlayer, null);
-				
-			$srcHeap := update($srcHeap, s#10, pacman$GameState.STATE, 6);
-			
-			// pacman.alloc = false
-			$srcHeap := update($srcHeap, pac#10, alloc, false);
-
+			call apply_Kill(todo);
 			// todo
-			assert (forall pac1: ref:: pac1 != null && dtype(pac1) == pacman$Pacman
-				==> !read($srcHeap, pac1, alloc));
+
 			
 			// exists RHS
 			
@@ -323,36 +259,14 @@ while(true)
 		
 	apply_UpdateFrame:
 		if(todo!=Seq#Empty()){
-			// execute applier block start
-			s#11 := Seq#Index(todo,0);
-			rec#11 := Seq#Index(todo,1);
-			pac#11 := Seq#Index(todo,2);
-
-
+		
 			// newRecord
 			havoc recordNew#11;
-			assume recordNew#11 != null && !read($srcHeap, recordNew#11, alloc) && dtype(recordNew#11) == 
-			pacman$Record;
-			$srcHeap := update($srcHeap, recordNew#11, alloc, true);
-			assume $IsGoodHeap($srcHeap);
-
-			
-			// gameState.STATE = 3
-			$srcHeap := update($srcHeap, s#11, pacman$GameState.STATE, 3);
-			
-			// gameState.record = newRecord
-			$srcHeap := update($srcHeap, s#11, pacman$GameState.record, recordNew#11);
-			
-			// initialize newRecord
-			$srcHeap := update($srcHeap, recordNew#11, pacman$Record.FRAME, read($srcHeap, rec#11, pacman$Record.FRAME)+1);
-			
-			$srcHeap := update($srcHeap, recordNew#11, pacman$Record.SCORE, read($srcHeap, rec#11, pacman$Record.SCORE));	
-
-			// rec.alloc = false
-			$srcHeap := update($srcHeap, rec#11, alloc, false);
-			
-
-			
+			assume recordNew#11 != null && !read($srcHeap, recordNew#11, alloc) && dtype(recordNew#11) == pacman$Record;
+	
+			// execute applier block start
+			call apply_UpdateFrame(todo, recordNew#11);
+					
 			// exists RHS
 			
 			// Termination Metric 
@@ -363,10 +277,6 @@ while(true)
 			goto nextRule;
 		}
 	
-
-
-	
-		
 	nextRule:	
 		goto survive;	
 
@@ -382,6 +292,7 @@ survive:
 
 
 }
+
 
 
 
