Prelude/SimpleGTRules.whole.bpl
@@ -1,0 +1,356 @@
+procedure match_PlayerMoveLeft() returns (res: Seq ref);
+ensures res==Seq#Empty() ==> (forall i: int :: inRange(i,0,Seq#Length(findPatterns_PlayerMoveLeft($srcHeap)))==>	
+!(   read($srcHeap,Seq#Index(Seq#Index(findPatterns_PlayerMoveLeft($srcHeap),i),0),pacman$GameState.STATE) == 3
+	 && read($srcHeap,Seq#Index(Seq#Index(findPatterns_PlayerMoveLeft($srcHeap),i),5),pacman$Action.DONEBY) == 1
+	 && read($srcHeap,Seq#Index(Seq#Index(findPatterns_PlayerMoveLeft($srcHeap),i),5),pacman$Action.FRAME) == 
+			read($srcHeap, Seq#Index(Seq#Index(findPatterns_PlayerMoveLeft($srcHeap),i),1), pacman$Record.FRAME)
+	 && read($srcHeap,Seq#Index(Seq#Index(findPatterns_PlayerMoveLeft($srcHeap),i),5),pacman$Action.DIRECTION)==1
+	 && !(dtype(read($srcHeap,Seq#Index(Seq#Index(findPatterns_PlayerMoveLeft($srcHeap),i),3), pacman$Grid.hasEnemy))<:pacman$Ghost)
+)
+);
+ensures res!=Seq#Empty() ==> 
+       Seq#Contains(findPatterns_PlayerMoveLeft($srcHeap), res) 
+	&& read($srcHeap,Seq#Index(res,0),pacman$GameState.STATE) == 3
+	&& read($srcHeap,Seq#Index(res,5),pacman$Action.DONEBY) == 1
+	&& read($srcHeap,Seq#Index(res,5),pacman$Action.FRAME) == 
+			read($srcHeap, Seq#Index(res,1), pacman$Record.FRAME)
+	&& read($srcHeap,Seq#Index(res,5),pacman$Action.DIRECTION)==1
+	&& !(dtype(read($srcHeap,Seq#Index(res,3), pacman$Grid.hasEnemy))<:pacman$Ghost)
+;
+
+procedure match_PlayerStay() returns (res: Seq ref);
+ensures res==Seq#Empty() ==> (forall i: int :: inRange(i,0,Seq#Length(findPatterns_PlayerStay($srcHeap)))==>	
+!(   read($srcHeap,Seq#Index(Seq#Index(findPatterns_PlayerStay($srcHeap),i),0),pacman$GameState.STATE) == 3
+	 && read($srcHeap,Seq#Index(Seq#Index(findPatterns_PlayerStay($srcHeap),i),4),pacman$Action.DONEBY) == 1
+	 && read($srcHeap,Seq#Index(Seq#Index(findPatterns_PlayerStay($srcHeap),i),4),pacman$Action.FRAME) == 
+			read($srcHeap, Seq#Index(Seq#Index(findPatterns_PlayerStay($srcHeap),i),1), pacman$Record.FRAME)
+	 && read($srcHeap,Seq#Index(Seq#Index(findPatterns_PlayerStay($srcHeap),i),4),pacman$Action.DIRECTION)==5
+
+)
+);
+ensures res!=Seq#Empty() ==> 
+       Seq#Contains(findPatterns_PlayerStay($srcHeap), res) 
+	&& read($srcHeap,Seq#Index(res,0),pacman$GameState.STATE) == 3
+	&& read($srcHeap,Seq#Index(res,4),pacman$Action.DONEBY) == 1
+	&& read($srcHeap,Seq#Index(res,4),pacman$Action.FRAME) == 
+			read($srcHeap, Seq#Index(res,1), pacman$Record.FRAME)
+	&& read($srcHeap,Seq#Index(res,4),pacman$Action.DIRECTION)==5
+;
+
+
+procedure match_GhostMoveLeft() returns (res: Seq ref);
+ensures res==Seq#Empty() ==> (forall i: int :: inRange(i,0,Seq#Length(findPatterns_GhostMoveLeft($srcHeap)))==>	
+!(   read($srcHeap,Seq#Index(Seq#Index(findPatterns_GhostMoveLeft($srcHeap),i),0),pacman$GameState.STATE) == 4
+	 && read($srcHeap,Seq#Index(Seq#Index(findPatterns_GhostMoveLeft($srcHeap),i),5),pacman$Action.DONEBY) == 2
+	 && read($srcHeap,Seq#Index(Seq#Index(findPatterns_GhostMoveLeft($srcHeap),i),5),pacman$Action.FRAME) == 
+			read($srcHeap, Seq#Index(Seq#Index(findPatterns_GhostMoveLeft($srcHeap),i),1), pacman$Record.FRAME)
+	 && read($srcHeap,Seq#Index(Seq#Index(findPatterns_GhostMoveLeft($srcHeap),i),5),pacman$Action.DIRECTION)==1)
+);
+ensures res!=Seq#Empty() ==> 
+       Seq#Contains(findPatterns_GhostMoveLeft($srcHeap), res) 
+	&& read($srcHeap,Seq#Index(res,0),pacman$GameState.STATE) == 4
+	&& read($srcHeap,Seq#Index(res,5),pacman$Action.DONEBY) == 2
+	&& read($srcHeap,Seq#Index(res,5),pacman$Action.FRAME) == 
+			read($srcHeap, Seq#Index(res,1), pacman$Record.FRAME)
+	&& read($srcHeap,Seq#Index(res,5),pacman$Action.DIRECTION)==1
+;
+
+procedure match_GhostStay() returns (res: Seq ref);
+ensures res==Seq#Empty() ==> (forall i: int :: inRange(i,0,Seq#Length(findPatterns_GhostStay($srcHeap)))==>	
+!(   read($srcHeap,Seq#Index(Seq#Index(findPatterns_GhostStay($srcHeap),i),0),pacman$GameState.STATE) == 4
+	 && read($srcHeap,Seq#Index(Seq#Index(findPatterns_GhostStay($srcHeap),i),4),pacman$Action.DONEBY) == 2
+	 && read($srcHeap,Seq#Index(Seq#Index(findPatterns_GhostStay($srcHeap),i),4),pacman$Action.FRAME) == 
+			read($srcHeap, Seq#Index(Seq#Index(findPatterns_GhostStay($srcHeap),i),1), pacman$Record.FRAME)
+	 && read($srcHeap,Seq#Index(Seq#Index(findPatterns_GhostStay($srcHeap),i),4),pacman$Action.DIRECTION)==5)
+);
+ensures res!=Seq#Empty() ==> 
+       Seq#Contains(findPatterns_GhostStay($srcHeap), res) 
+	&& read($srcHeap,Seq#Index(res,0),pacman$GameState.STATE) == 4
+	&& read($srcHeap,Seq#Index(res,4),pacman$Action.DONEBY) == 2
+	&& read($srcHeap,Seq#Index(res,4),pacman$Action.FRAME) == 
+			read($srcHeap, Seq#Index(res,1), pacman$Record.FRAME)
+	&& read($srcHeap,Seq#Index(res,4),pacman$Action.DIRECTION)==5
+;
+
+procedure match_Collect() returns (res: Seq ref);
+ensures res==Seq#Empty() ==> (forall i: int :: inRange(i,0,Seq#Length(findPatterns_Collect($srcHeap)))==>	
+!(  read($srcHeap,Seq#Index(Seq#Index(findPatterns_Collect($srcHeap),i),0),pacman$GameState.STATE) == 5
+));
+ensures res!=Seq#Empty() ==> 
+       Seq#Contains(findPatterns_Collect($srcHeap), res) 
+	&& read($srcHeap,Seq#Index(res,0),pacman$GameState.STATE) == 5
+;
+
+procedure match_Kill() returns (res: Seq ref);
+ensures res==Seq#Empty() ==> (forall i: int :: inRange(i,0,Seq#Length(findPatterns_Kill($srcHeap)))==>	
+!(  read($srcHeap,Seq#Index(Seq#Index(findPatterns_Kill($srcHeap),i),0),pacman$GameState.STATE) == 5
+));
+ensures res!=Seq#Empty() ==> 
+       Seq#Contains(findPatterns_Kill($srcHeap), res) 
+	&& read($srcHeap,Seq#Index(res,0),pacman$GameState.STATE) == 5
+;
+
+procedure match_UpdateFrame() returns (res: Seq ref);
+ensures res==Seq#Empty() ==> (forall i: int :: inRange(i,0,Seq#Length(findPatterns_UpdateFrame($srcHeap)))==>	
+!(  read($srcHeap,Seq#Index(Seq#Index(findPatterns_UpdateFrame($srcHeap),i),0),pacman$GameState.STATE) == 5 
+));
+ensures res!=Seq#Empty() ==> 
+       Seq#Contains(findPatterns_UpdateFrame($srcHeap), res) 
+	&& read($srcHeap,Seq#Index(res,0),pacman$GameState.STATE) == 5
+;
+
+
+procedure apply_PlayerMoveLeft(res: Seq ref);
+requires $Well_form($srcHeap);
+requires lemma_col($srcHeap, col);
+requires Seq#Contains(findPatterns_PlayerMoveLeft($srcHeap), res) 
+   && read($srcHeap,Seq#Index(res,0),pacman$GameState.STATE) == 3
+   && read($srcHeap,Seq#Index(res,5),pacman$Action.DONEBY) == 1
+   && read($srcHeap,Seq#Index(res,5),pacman$Action.FRAME) == 
+      read($srcHeap, Seq#Index(res,1), pacman$Record.FRAME)
+   && read($srcHeap,Seq#Index(res,5),pacman$Action.DIRECTION)==1
+   && !(dtype(read($srcHeap,Seq#Index(res,3), pacman$Grid.hasEnemy))<:pacman$Ghost);
+modifies $srcHeap, col;
+// s : P!GameState(STATE=~4)
+ensures read($srcHeap,Seq#Index(res,0),pacman$GameState.STATE) == 4;
+// grid2: P!Grid(hasPlayer=~pac)
+ensures read($srcHeap,Seq#Index(res,3),pacman$Grid.hasPlayer) == Seq#Index(res,2);
+// grid1: P!Grid(hasPlayer=~null)
+ensures read($srcHeap,Seq#Index(res,4),pacman$Grid.hasPlayer) == null;
+// act : P!Action(alloc=~false)
+ensures !read($srcHeap,Seq#Index(res,5),alloc);
+ensures (forall<alpha> o:ref,f:Field alpha::
+  o!=null && read(old($srcHeap),o,alloc)==>
+   (dtype(o)==pacman$GameState && f==pacman$GameState.STATE)
+   ||(dtype(o)==pacman$Grid && f==pacman$Grid.hasPlayer)
+   ||(dtype(o)==pacman$Action && (f==alloc||f==pacman$Action.DONEBY||f==pacman$Action.DIRECTION		||f==pacman$Action.FRAME))
+   ||(read($srcHeap,o,f)==read(old($srcHeap),o,f))); 
+ensures  $Well_form($srcHeap);
+ensures lemma_col($srcHeap, col);
+
+procedure apply_PlayerStay(res: Seq ref);
+requires $Well_form($srcHeap);
+requires lemma_col($srcHeap, col);
+requires Seq#Contains(findPatterns_PlayerStay($srcHeap), res) 
+	&& read($srcHeap,Seq#Index(res,0),pacman$GameState.STATE) == 3
+	&& read($srcHeap,Seq#Index(res,4),pacman$Action.DONEBY) == 1
+	&& read($srcHeap,Seq#Index(res,4),pacman$Action.FRAME) == 
+			read($srcHeap, Seq#Index(res,1), pacman$Record.FRAME)
+	&& read($srcHeap,Seq#Index(res,4),pacman$Action.DIRECTION)==5;
+modifies $srcHeap;
+ensures read($srcHeap, Seq#Index(res,0), pacman$GameState.STATE)==4;
+ensures !read($srcHeap, Seq#Index(res,4), alloc);
+ensures (forall<alpha> o:ref,f:Field alpha::
+  o!=null && read(old($srcHeap),o,alloc)==>
+   (dtype(o)==pacman$GameState && f==pacman$GameState.STATE)
+   ||(dtype(o)==pacman$Action && (f==alloc||f==pacman$Action.DONEBY||f==pacman$Action.DIRECTION		||f==pacman$Action.FRAME))
+   ||(read($srcHeap,o,f)==read(old($srcHeap),o,f))); 
+ensures $Well_form($srcHeap);
+ensures lemma_col($srcHeap, col);
+ 
+procedure apply_GhostMoveLeft(res: Seq ref);
+requires $Well_form($srcHeap);
+requires lemma_col($srcHeap, col);
+requires Seq#Contains(findPatterns_GhostMoveLeft($srcHeap), res) 
+	&& read($srcHeap,Seq#Index(res,0),pacman$GameState.STATE) == 4
+	&& read($srcHeap,Seq#Index(res,5),pacman$Action.DONEBY) == 2
+	&& read($srcHeap,Seq#Index(res,5),pacman$Action.FRAME) == 
+			read($srcHeap, Seq#Index(res,1), pacman$Record.FRAME)
+	&& read($srcHeap,Seq#Index(res,5),pacman$Action.DIRECTION)==1;
+modifies $srcHeap;
+// s : P!GameState(STATE=~5)
+ensures read($srcHeap,Seq#Index(res,0),pacman$GameState.STATE) == 5;
+// grid2: P!Grid(hasEnemy=~ghost)
+ensures read($srcHeap,Seq#Index(res,3),pacman$Grid.hasEnemy) == Seq#Index(res,2);
+// grid1: P!Grid(hasEnemy=~null)
+ensures read($srcHeap,Seq#Index(res,4),pacman$Grid.hasEnemy) == null;
+// act : P!Action(alloc=~false)
+ensures !read($srcHeap,Seq#Index(res,5),alloc);
+ensures (forall<alpha> o:ref,f:Field alpha::
+  o!=null && read(old($srcHeap),o,alloc)==>
+   (dtype(o)==pacman$GameState && f==pacman$GameState.STATE)
+   ||(dtype(o)==pacman$Grid && f==pacman$Grid.hasEnemy)
+   ||(dtype(o)==pacman$Action && (f==alloc||f==pacman$Action.DONEBY||f==pacman$Action.DIRECTION		||f==pacman$Action.FRAME))
+   ||(read($srcHeap,o,f)==read(old($srcHeap),o,f))); 
+ensures  $Well_form($srcHeap);
+ensures  lemma_col($srcHeap, col);
+
+procedure apply_GhostStay(res: Seq ref);
+requires $Well_form($srcHeap);
+requires lemma_col($srcHeap, col);
+requires Seq#Contains(findPatterns_GhostStay($srcHeap), res) 
+	&& read($srcHeap,Seq#Index(res,0),pacman$GameState.STATE) == 4
+	&& read($srcHeap,Seq#Index(res,4),pacman$Action.DONEBY) == 2
+	&& read($srcHeap,Seq#Index(res,4),pacman$Action.FRAME) == 
+			read($srcHeap, Seq#Index(res,1), pacman$Record.FRAME)
+	&& read($srcHeap,Seq#Index(res,4),pacman$Action.DIRECTION)==5 ;
+modifies $srcHeap;
+ensures read($srcHeap, Seq#Index(res,0), pacman$GameState.STATE)==5;
+ensures !read($srcHeap, Seq#Index(res,4), alloc);
+ensures (forall<alpha> o:ref,f:Field alpha::
+  o!=null && read(old($srcHeap),o,alloc)==>
+   (dtype(o)==pacman$GameState && f==pacman$GameState.STATE)
+   ||(dtype(o)==pacman$Action && (f==alloc||f==pacman$Action.DONEBY||f==pacman$Action.DIRECTION	||f==pacman$Action.FRAME))
+   ||(read($srcHeap,o,f)==read(old($srcHeap),o,f))); 
+ensures $Well_form($srcHeap);
+ensures lemma_col($srcHeap, col);
+ 
+procedure apply_Collect(res: Seq ref, recNew: ref);
+requires $Well_form($srcHeap);
+requires lemma_col($srcHeap, col);
+requires Seq#Contains(findPatterns_Collect($srcHeap), res) 
+	&& read($srcHeap,Seq#Index(res,0),pacman$GameState.STATE) == 5
+	&& recNew!=null && !read($srcHeap,recNew,alloc) && dtype(recNew)==pacman$Record;
+modifies $srcHeap;
+ensures recNew!=null && read($srcHeap,recNew,alloc) && dtype(recNew)==pacman$Record;
+// gameState.record = newRecord
+ensures read($srcHeap, Seq#Index(res,0), pacman$GameState.record) == recNew;
+// initialize newRecord
+ensures read($srcHeap, recNew, pacman$Record.FRAME) == old(read($srcHeap, Seq#Index(res,1), pacman$Record.FRAME));
+ensures read($srcHeap, recNew, pacman$Record.SCORE) == old(read($srcHeap, Seq#Index(res,1), pacman$Record.SCORE)+100);
+// Grid.hasGem = null
+ensures read($srcHeap, Seq#Index(res,4), pacman$Grid.hasGem) == null;
+// gem.alloc = false
+ensures !read($srcHeap, Seq#Index(res,3), alloc);
+// rec.alloc = false
+ensures !read($srcHeap, Seq#Index(res,1), alloc);
+ensures (forall<alpha> o:ref,f:Field alpha::
+  o!=null && read(old($srcHeap),o,alloc)==>
+   (dtype(o)==pacman$GameState && (f==pacman$GameState.STATE||f==pacman$GameState.record))
+   ||(dtype(o)==pacman$Grid && f==pacman$Grid.hasGem)
+   ||(dtype(o)==pacman$Record && (f==pacman$Record.FRAME||f==pacman$Record.SCORE||f==alloc))
+   ||(dtype(o)==pacman$Gem && f==alloc)
+   ||(read($srcHeap,o,f)==read(old($srcHeap),o,f))); 
+ensures  $Well_form($srcHeap);   
+ensures  lemma_col($srcHeap, col);
+   
+procedure apply_Kill(res: Seq ref);
+requires $Well_form($srcHeap);
+requires lemma_col($srcHeap, col);
+requires Seq#Contains(findPatterns_Kill($srcHeap), res) 
+	&& read($srcHeap,Seq#Index(res,0),pacman$GameState.STATE) == 5;
+modifies $srcHeap;
+// GameState.STATE = 6		
+ensures read($srcHeap, Seq#Index(res,0), pacman$GameState.STATE)==6;
+// Grid.hasPlayer = null
+ensures read($srcHeap, Seq#Index(res,3), pacman$Grid.hasPlayer)==null;		
+// pacman.alloc = false
+ensures !read($srcHeap, Seq#Index(res,2), alloc);
+ensures (forall<alpha> o:ref,f:Field alpha::
+  o!=null && read(old($srcHeap),o,alloc)==>
+   (dtype(o)==pacman$GameState && (f==pacman$GameState.STATE))
+   ||(dtype(o)==pacman$Grid && f==pacman$Grid.hasPlayer)
+   ||(dtype(o)==pacman$Pacman && f==alloc)
+   ||(read($srcHeap,o,f)==read(old($srcHeap),o,f)));
+ensures  $Well_form($srcHeap);
+ensures  lemma_col($srcHeap, col);
+
+procedure apply_UpdateFrame(res: Seq ref, recNew: ref);
+requires $Well_form($srcHeap);
+requires lemma_col($srcHeap, col);
+requires  Seq#Contains(findPatterns_UpdateFrame($srcHeap), res) 
+	&& read($srcHeap,Seq#Index(res,0),pacman$GameState.STATE) == 5
+	&& recNew!=null && !read($srcHeap,recNew,alloc) && dtype(recNew)==pacman$Record;
+modifies $srcHeap;
+ensures recNew!=null && read($srcHeap,recNew,alloc) && dtype(recNew)==pacman$Record;
+// gameState.STATE = 3
+ensures read($srcHeap, Seq#Index(res,0), pacman$GameState.STATE) == 3;		
+// gameState.record = newRecord
+ensures read($srcHeap, Seq#Index(res,0), pacman$GameState.record) == recNew;		
+// initialize newRecord
+ensures read($srcHeap, recNew, pacman$Record.FRAME) == old(read($srcHeap, Seq#Index(res,1), pacman$Record.FRAME)+1);
+ensures read($srcHeap, recNew, pacman$Record.SCORE) == old(read($srcHeap, Seq#Index(res,1), pacman$Record.SCORE));	
+// rec.alloc = false
+ensures !read($srcHeap, Seq#Index(res,1), alloc);
+ensures (forall<alpha> o:ref,f:Field alpha::
+  o!=null && read(old($srcHeap),o,alloc)==>
+   (dtype(o)==pacman$GameState && (f==pacman$GameState.STATE||f==pacman$GameState.record))
+   ||(dtype(o)==pacman$Record && (f==pacman$Record.FRAME||f==pacman$Record.SCORE||f==alloc))
+   ||(read($srcHeap,o,f)==read(old($srcHeap),o,f)));
+ensures  $Well_form($srcHeap);
+ensures  lemma_col($srcHeap, col);
+
+
+
+function $Well_form($hp:HeapType): bool
+{
+// 1.
+(forall pac1,pac2: ref::
+	pac1 != null && read($hp,pac1,alloc) && dtype(pac1) == pacman$Pacman
+&&	pac2 != null && read($hp,pac2,alloc) && dtype(pac2) == pacman$Pacman
+==>
+	pac1 == pac2
+) 
+&&
+// 2.
+(forall r1,r2: ref::
+	r1 != null && read($hp,r1,alloc) && dtype(r1) == pacman$Record
+&&	r2 != null && read($hp,r2,alloc) && dtype(r2) == pacman$Record
+==>
+	r1 ==r2
+)
+&&
+// 3.
+(forall<alpha> grid1, grid2: ref :: 
+	grid1 != null && read($hp,grid1,alloc) && dtype(grid1) == pacman$Grid
+&&	grid2 != null && read($hp,grid2,alloc) && dtype(grid2) == pacman$Grid
+	/* grid1 can equal to grid2 */
+	==>
+	reachable($hp, grid1, grid2)
+)
+&&
+// 4.
+(forall gs1,gs2: ref::
+	gs1 != null && read($hp,gs1,alloc) && dtype(gs1) == pacman$GameState
+&&	gs2 != null && read($hp,gs2,alloc) && dtype(gs2) == pacman$GameState
+==>
+	gs1 == gs2
+)
+&&
+// 5.
+(forall gs1: ref::
+	(gs1 != null && read($hp,gs1,alloc) && dtype(gs1) == pacman$GameState && read($hp,gs1,pacman$GameState.STATE)==3) ==>
+	(forall<alpha> grid1: ref :: grid1 != null && read($hp,grid1,alloc) && dtype(grid1) == pacman$Grid && dtype(read($hp,grid1,pacman$Grid.hasEnemy)) <: pacman$Ghost
+		==> !(dtype(read($hp,grid1,pacman$Grid.hasPlayer)) <: pacman$Pacman) ))
+&&
+// 6.
+(forall gs1: ref::
+	(gs1 != null && read($hp,gs1,alloc) && dtype(gs1) == pacman$GameState && read($hp,gs1,pacman$GameState.STATE)==4) ==>
+	(forall<alpha> grid1: ref :: grid1 != null && read($hp,grid1,alloc) && dtype(grid1) == pacman$Grid && dtype(read($hp,grid1,pacman$Grid.hasEnemy)) <: pacman$Ghost
+		==> !(dtype(read($hp,grid1,pacman$Grid.hasPlayer)) <: pacman$Pacman) ))
+}
+
+var col: Seq ref;
+var idx: int;
+
+	
+
+
+function lemma_col($hp: HeapType, $col: Seq ref):bool
+{
+(forall i: int :: 0<=i && i<Seq#Length($col) ==>
+Seq#Index($col,i) != null 
+&& read($hp, Seq#Index($col,i), alloc) 
+&& dtype(Seq#Index($col,i)) == pacman$Action
+&& read($hp, Seq#Index($col,i), pacman$Action.DONEBY) == 1
+&& read($hp, Seq#Index($col,i), pacman$Action.DIRECTION) != 5
+)
+&&
+(forall i: int :: 0<=i && i<Seq#Length($col)-1 ==>
+	read($hp, Seq#Index($col,i+1), pacman$Action.FRAME) - read($hp, Seq#Index($col,i), pacman$Action.FRAME) < Pacman#ghost#INTERVAL	
+)
+&&
+(forall i,j: int :: 0<=i && i<j && j<Seq#Length($col) ==>
+	Seq#Index($col,i)!=Seq#Index($col,j)
+)
+}
+
+/*
+&&
+(forall<alpha> grid: ref :: 
+	grid != null && read($hp,grid,alloc) && dtype(grid) == pacman$Grid
+	&& read($hp,grid,pacman$Grid.hasGem)!=null && read($hp,read($hp,grid,pacman$Grid.hasGem),alloc)
+	==>
+	dtype(read($hp,grid,pacman$Grid.hasGem)) == pacman$Gem
+)
+*/
