Rule_TranslationValidation/apply_Collect.bpl
@@ -1,0 +1,145 @@
+procedure apply_CollectTest(res: Seq ref, recNew: ref)
+requires $Well_form($srcHeap);
+requires lemma_col($srcHeap, col);
+requires Seq#Contains(findPatterns_Collect($srcHeap), res) 
+	&& read($srcHeap,Seq#Index(res,0),pacman$GameState.STATE) == 5
+	&& recNew!=null && !read($srcHeap,recNew,alloc) && dtype(recNew)==pacman$Record;
+modifies $srcHeap;
+ensures recNew!=null && read($srcHeap,recNew,alloc) && dtype(recNew)==pacman$Record;
+// gameState.record = newRecord
+ensures read($srcHeap, Seq#Index(res,0), pacman$GameState.record) == recNew;
+// initialize newRecord
+ensures read($srcHeap, recNew, pacman$Record.FRAME) == old(read($srcHeap, Seq#Index(res,1), pacman$Record.FRAME));
+ensures read($srcHeap, recNew, pacman$Record.SCORE) == old(read($srcHeap, Seq#Index(res,1), pacman$Record.SCORE)+100);
+// Grid.hasGem = null
+ensures read($srcHeap, Seq#Index(res,4), pacman$Grid.hasGem) == null;
+// gem.alloc = false
+ensures !read($srcHeap, Seq#Index(res,3), alloc);
+// rec.alloc = false
+ensures !read($srcHeap, Seq#Index(res,1), alloc);
+ensures (forall<alpha> o:ref,f:Field alpha::
+  o!=null && read(old($srcHeap),o,alloc)==>
+   (dtype(o)==pacman$GameState && (f==pacman$GameState.STATE||f==pacman$GameState.record))
+   ||(dtype(o)==pacman$Grid && f==pacman$Grid.hasGem)
+   ||(dtype(o)==pacman$Record && (f==pacman$Record.FRAME||f==pacman$Record.SCORE||f==alloc))
+   ||(dtype(o)==pacman$Gem && f==alloc)
+   ||(read($srcHeap,o,f)==read(old($srcHeap),o,f))); 
+ensures $Well_form($srcHeap);
+ensures lemma_col($srcHeap, col);
+{
+	var s#9: ref;
+	var rec#9: ref;
+	var pac#9: ref;
+	var gem#9: ref;
+	var grid#9: ref;
+	var recordNew#9: ref;
+	var stk: Seq BoxType;
+	
+	
+	// allocation
+	$srcHeap := update($srcHeap, recNew, alloc, true);
+	assume $IsGoodHeap($srcHeap);
+	
+	// local init
+	s#9 := Seq#Index(res,0);
+	rec#9 := Seq#Index(res,1);
+	pac#9 := Seq#Index(res,2);
+	gem#9 := Seq#Index(res,3);
+	grid#9 := Seq#Index(res,4);
+	recordNew#9 := recNew;
+	
+	// stk init
+	stk := OpCode#Aux#InitStk();
+			
+	 // 0: LOAD 0, 1 (s: P!GameState)
+	 call stk := OpCode#Load(stk, s#9);
+	 // 1: LOAD 0, 2 (rec: P!Record)
+	 call stk := OpCode#Load(stk, rec#9);
+	 // 2: REMOVE (fieldname: record)
+	 assert Seq#Length(stk) >= 2;
+	 assert $Unbox(Seq#Index(stk, Seq#Length(stk)-2)) != null;
+	
+	 $srcHeap := update($srcHeap, $Unbox(Seq#Index(stk, Seq#Length(stk)-2)),FieldOfDecl(dtype($Unbox(Seq#Index(stk, Seq#Length(stk)-2))), _Field$record): Field (ref),null);
+	 
+	 stk := Seq#Take(stk, Seq#Length(stk)-2);
+	 // 3: LOAD 0, 5 (grid: P!Grid)
+	 call stk := OpCode#Load(stk, grid#9);
+	 // 4: LOAD 0, 4 (gem: P!Gem)
+	 call stk := OpCode#Load(stk, gem#9);
+	 // 5: REMOVE (fieldname: hasGem)
+	 assert Seq#Length(stk) >= 2;
+	 assert $Unbox(Seq#Index(stk, Seq#Length(stk)-2)) != null;
+	
+	 $srcHeap := update($srcHeap, $Unbox(Seq#Index(stk, Seq#Length(stk)-2)),FieldOfDecl(dtype($Unbox(Seq#Index(stk, Seq#Length(stk)-2))), _Field$hasGem): Field (ref),null);
+	 
+	 stk := Seq#Take(stk, Seq#Length(stk)-2);
+	 // 6: LOAD 0, 1 (s: P!GameState)
+	 call stk := OpCode#Load(stk, s#9);
+	 // 7: LOAD 0, 6 (recNew: P!Record)
+	 call stk := OpCode#Load(stk, recordNew#9);
+	 // 8: ADD (fieldname: record)
+	 assert Seq#Length(stk) >= 2;
+	 assert $Unbox(Seq#Index(stk, Seq#Length(stk)-2)) != null;
+
+	 
+	 $srcHeap := update($srcHeap, $Unbox(Seq#Index(stk, Seq#Length(stk)-2)), FieldOfDecl(dtype($Unbox(Seq#Index(stk, Seq#Length(stk)-2))), _Field$record): Field (ref), $Unbox(Seq#Index(stk, Seq#Length(stk)-1)));
+	 
+	 stk := Seq#Take(stk, Seq#Length(stk)-2); 
+	 // 9: LOAD 0, 6 (recNew: P!Record)
+	call stk := OpCode#Load(stk, recordNew#9);
+	// 10: LOAD 0, 2 (rec: P!Record)
+	call stk := OpCode#Load(stk, rec#9);
+	// 11: GET (fieldname: FRAME)
+	assert Seq#Length(stk) >= 1;
+	assert $Unbox(Seq#Index(stk, Seq#Length(stk)-1)) != null;
+	stk := Seq#Build(Seq#Take(stk, Seq#Length(stk)-1), $Box($srcHeap[$Unbox(Seq#Index(stk, Seq#Length(stk)-1)), FieldOfDecl(dtype($Unbox(Seq#Index(stk, Seq#Length(stk)-1))), _Field$FRAME): Field (int)]));
+	// 12: ADD (fieldname: FRAME)
+	 assert Seq#Length(stk) >= 2;
+	 assert $Unbox(Seq#Index(stk, Seq#Length(stk)-2)) != null;
+
+	 
+	 $srcHeap := update($srcHeap, $Unbox(Seq#Index(stk, Seq#Length(stk)-2)), FieldOfDecl(dtype($Unbox(Seq#Index(stk, Seq#Length(stk)-2))), _Field$FRAME): Field (int), $Unbox(Seq#Index(stk, Seq#Length(stk)-1)));
+	 
+	 stk := Seq#Take(stk, Seq#Length(stk)-2); 
+	// 13: LOAD 0, 6 (recNew: P!Record)
+	call stk := OpCode#Load(stk, recordNew#9);
+	// 14: LOAD 0, 2 (rec: P!Record)
+	call stk := OpCode#Load(stk, rec#9);
+	// 15: GET (fieldname: SCORE)
+	assert Seq#Length(stk) >= 1;
+	assert $Unbox(Seq#Index(stk, Seq#Length(stk)-1)) != null;
+	stk := Seq#Build(Seq#Take(stk, Seq#Length(stk)-1), $Box($srcHeap[$Unbox(Seq#Index(stk, Seq#Length(stk)-1)), FieldOfDecl(dtype($Unbox(Seq#Index(stk, Seq#Length(stk)-1))), _Field$SCORE): Field (int)]));
+	// 16: PUSH (intValue: 100)
+	call stk := OpCode#Pushi(stk, 100);
+	// 17: INVOKE (argcount: 1) (opname: +)
+	call stk := OCL#Integer#Plus(stk);
+	// 18: ADD (fieldname: SCORE)
+	 assert Seq#Length(stk) >= 2;
+	 assert $Unbox(Seq#Index(stk, Seq#Length(stk)-2)) != null;
+
+	 $srcHeap := update($srcHeap, $Unbox(Seq#Index(stk, Seq#Length(stk)-2)), FieldOfDecl(dtype($Unbox(Seq#Index(stk, Seq#Length(stk)-2))), _Field$SCORE): Field (int), $Unbox(Seq#Index(stk, Seq#Length(stk)-1)));
+	 
+	 stk := Seq#Take(stk, Seq#Length(stk)-2); 
+	// 19: LOAD 0, 2 (rec: P!Record)
+	call stk := OpCode#Load(stk, rec#9);
+	// 20: DELETE
+	assert Seq#Length(stk) >= 1;
+	assert $Unbox(OpCode#Top(stk)) != null;
+	$srcHeap := update($srcHeap, $Unbox(OpCode#Top(stk)), alloc, false);
+	stk := Seq#Take(stk, Seq#Length(stk)-1);	
+	// 21: LOAD 0, 4 (gem: P!Gem)
+	call stk := OpCode#Load(stk, gem#9);
+	// 22: DELETE	
+	assert Seq#Length(stk) >= 1;
+	assert $Unbox(OpCode#Top(stk)) != null;
+	$srcHeap := update($srcHeap, $Unbox(OpCode#Top(stk)), alloc, false);
+	stk := Seq#Take(stk, Seq#Length(stk)-1);	
+
+	
+
+	
+
+	
+
+
+}
