Rule_TranslationValidation/apply_Kill.bpl
@@ -1,0 +1,75 @@
+procedure apply_KillTest(res: Seq ref)
+requires $Well_form($srcHeap);
+requires lemma_col($srcHeap, col);
+requires Seq#Contains(findPatterns_Kill($srcHeap), res) 
+	&& read($srcHeap,Seq#Index(res,0),pacman$GameState.STATE) == 5;
+modifies $srcHeap;
+// GameState.STATE = 6		
+ensures read($srcHeap, Seq#Index(res,0), pacman$GameState.STATE)==6;
+// Grid.hasPlayer = null
+ensures read($srcHeap, Seq#Index(res,3), pacman$Grid.hasPlayer)==null;		
+// pacman.alloc = false
+ensures !read($srcHeap, Seq#Index(res,2), alloc);
+ensures (forall<alpha> o:ref,f:Field alpha::
+  o!=null && read(old($srcHeap),o,alloc)==>
+   (dtype(o)==pacman$GameState && (f==pacman$GameState.STATE))
+   ||(dtype(o)==pacman$Grid && f==pacman$Grid.hasPlayer)
+   ||(dtype(o)==pacman$Pacman && f==alloc)
+   ||(read($srcHeap,o,f)==read(old($srcHeap),o,f)));
+ensures $Well_form($srcHeap);
+ensures lemma_col($srcHeap, col);
+{
+	var s#10: ref;
+	var ghost#10: ref;
+	var pac#10: ref;
+	var grid#10: ref;
+	var stk: Seq BoxType;
+	
+	s#10 := Seq#Index(res,0);
+	ghost#10 := Seq#Index(res,1);
+	pac#10 := Seq#Index(res,2);
+	grid#10 := Seq#Index(res,3);
+
+	stk := OpCode#Aux#InitStk();
+	
+	 // 0: LOAD 0, 1 (s: P!GameState)
+	 call stk := OpCode#Load(stk, s#10);
+	 // 1: PUSH (intValue: 5)
+	 call stk := OpCode#Pushi(stk, 5);
+	 // 2: REMOVE (fieldname: STATE)
+	 assert Seq#Length(stk) >= 2;
+	 assert $Unbox(Seq#Index(stk, Seq#Length(stk)-2)) != null;
+	
+	 $srcHeap := update($srcHeap, $Unbox(Seq#Index(stk, Seq#Length(stk)-2)),FieldOfDecl(dtype($Unbox(Seq#Index(stk, Seq#Length(stk)-2))), _Field$STATE): Field (int),0);
+	 
+	 stk := Seq#Take(stk, Seq#Length(stk)-2);
+	 // 3: LOAD 0, 4 (grid: P!Grid)
+	 call stk := OpCode#Load(stk, grid#10);
+	 // 4: LOAD 0, 3 (pac: P!Pacman)
+	 call stk := OpCode#Load(stk, pac#10);
+	 // 5: REMOVE (fieldname: hasPlayer)
+	 assert Seq#Length(stk) >= 2;
+	 assert $Unbox(Seq#Index(stk, Seq#Length(stk)-2)) != null;
+	
+	 $srcHeap := update($srcHeap, $Unbox(Seq#Index(stk, Seq#Length(stk)-2)),FieldOfDecl(dtype($Unbox(Seq#Index(stk, Seq#Length(stk)-2))), _Field$hasPlayer): Field (ref),null);
+	 
+	 stk := Seq#Take(stk, Seq#Length(stk)-2);
+	 // 6: LOAD 0, 1 (s: P!GameState)
+	 call stk := OpCode#Load(stk, s#10);
+	 // 7: PUSH (intValue: 6)
+	 call stk := OpCode#Pushi(stk, 6);
+	 // 8: ADD (fieldname: STATE)
+	 assert Seq#Length(stk) >= 2;
+	 assert $Unbox(Seq#Index(stk, Seq#Length(stk)-2)) != null;
+
+	 $srcHeap := update($srcHeap, $Unbox(Seq#Index(stk, Seq#Length(stk)-2)), FieldOfDecl(dtype($Unbox(Seq#Index(stk, Seq#Length(stk)-2))), _Field$STATE): Field (int), $Unbox(Seq#Index(stk, Seq#Length(stk)-1)));
+	 
+	 stk := Seq#Take(stk, Seq#Length(stk)-2); 	 
+	 // 9: LOAD 0, 3 (pac: P!Pacman)
+	call stk := OpCode#Load(stk, pac#10);
+	// 10: DELETE
+	assert Seq#Length(stk) >= 1;
+	assert $Unbox(OpCode#Top(stk)) != null;
+	$srcHeap := update($srcHeap, $Unbox(OpCode#Top(stk)), alloc, false);
+	stk := Seq#Take(stk, Seq#Length(stk)-1);	
+}
