Rule_TranslationValidation/match_GhostStay.bpl
@@ -1,0 +1,194 @@
+procedure match_GhostStayTest() returns (res: Seq ref)
+ensures res==Seq#Empty() ==> (forall i: int :: inRange(i,0,Seq#Length(findPatterns_GhostStay($srcHeap)))==>	
+!(   read($srcHeap,Seq#Index(Seq#Index(findPatterns_GhostStay($srcHeap),i),0),pacman$GameState.STATE) == 4
+	 && read($srcHeap,Seq#Index(Seq#Index(findPatterns_GhostStay($srcHeap),i),4),pacman$Action.DONEBY) == 2
+	 && read($srcHeap,Seq#Index(Seq#Index(findPatterns_GhostStay($srcHeap),i),4),pacman$Action.FRAME) == 
+			read($srcHeap, Seq#Index(Seq#Index(findPatterns_GhostStay($srcHeap),i),1), pacman$Record.FRAME)
+	 && read($srcHeap,Seq#Index(Seq#Index(findPatterns_GhostStay($srcHeap),i),4),pacman$Action.DIRECTION)==5)
+);
+ensures res!=Seq#Empty() ==> 
+       Seq#Contains(findPatterns_GhostStay($srcHeap), res) 
+	&& read($srcHeap,Seq#Index(res,0),pacman$GameState.STATE) == 4
+	&& read($srcHeap,Seq#Index(res,4),pacman$Action.DONEBY) == 2
+	&& read($srcHeap,Seq#Index(res,4),pacman$Action.FRAME) == 
+			read($srcHeap, Seq#Index(res,1), pacman$Record.FRAME)
+	&& read($srcHeap,Seq#Index(res,4),pacman$Action.DIRECTION)==5
+;
+{
+var $i: int;
+
+var s#8: ref;
+var rec#8: ref;
+var ghost#8: ref;
+var grid1#8: ref;
+var act#8: ref;
+
+var P#8: Seq (Seq ref);
+var b#8: bool;
+
+var cursor: Seq ref;
+
+
+		P#8 := findPatterns_GhostStay($srcHeap);
+
+		$i := 0;
+		res := Seq#Empty();
+		while($i < Seq#Length(P#8))
+			invariant $i <= Seq#Length(P#8);
+			invariant (forall i: int :: inRange(i,0,$i)==>	
+		      !(read($srcHeap,Seq#Index(Seq#Index(P#8,i),0),pacman$GameState.STATE) == 4
+			 && read($srcHeap,Seq#Index(Seq#Index(P#8,i),4),pacman$Action.DONEBY) == 2
+			 && read($srcHeap,Seq#Index(Seq#Index(P#8,i),4),pacman$Action.FRAME) == 
+					read($srcHeap, Seq#Index(Seq#Index(P#8,i),1), pacman$Record.FRAME)
+			 && read($srcHeap,Seq#Index(Seq#Index(P#8,i),4),pacman$Action.DIRECTION)==5)
+			);
+		{
+
+			cursor := Seq#Index(P#8, $i);
+			
+			s#8 := Seq#Index(cursor,0);
+			rec#8 := Seq#Index(cursor,1);
+			ghost#8 := Seq#Index(cursor,2);
+			grid1#8 := Seq#Index(cursor,3);
+			act#8 := Seq#Index(cursor,4);
+
+			// conditional filter
+			call b#8 := match_filter_GhostStay(s#8,rec#8,ghost#8,grid1#8,act#8);		
+			
+			// check filter and NAC;
+
+			if(b#8){res := cursor; break;}
+			$i := $i+1;
+		}
+
+
+}
+
+
+
+
+
+procedure match_filter_GhostStay(s:ref, rec:ref, ghost:ref, grid1:ref, act:ref) returns(r: bool)
+ requires s != null && read($srcHeap,s,alloc) && dtype(s) == pacman$GameState;
+ requires rec != null && read($srcHeap,rec,alloc) && dtype(rec) == pacman$Record;
+ requires ghost != null && read($srcHeap,ghost,alloc) && dtype(ghost) == pacman$Ghost;
+ requires grid1 != null && read($srcHeap,grid1,alloc) && dtype(grid1) == pacman$Grid;
+ requires act != null && read($srcHeap,act,alloc) && dtype(act) == pacman$Action;
+ requires read($srcHeap,s,pacman$GameState.record) == rec;
+ requires read($srcHeap,grid1,pacman$Grid.hasEnemy) == ghost;
+ ensures r <==> ( 
+		read($srcHeap,s,pacman$GameState.STATE) == 4
+	 && read($srcHeap,act,pacman$Action.DONEBY) == 2
+	 && read($srcHeap,act,pacman$Action.FRAME) == read($srcHeap, rec, pacman$Record.FRAME)
+	 && read($srcHeap,act,pacman$Action.DIRECTION)==5);
+{
+
+var s#8: ref;
+var rec#8: ref;
+var ghost#8: ref;
+var grid1#8: ref;
+var act#8: ref;
+var stk: Seq BoxType;
+
+var b#4: bool;
+var b#11: bool;
+var b#19: bool;
+
+var b#4#Box: BoxType;
+var b#11#Box: BoxType;
+var b#19#Box: BoxType;
+
+s#8,rec#8,ghost#8,grid1#8,act#8 := s, rec, ghost, grid1, act;
+
+stk := OpCode#Aux#InitStk();
+
+Label_0:
+	 // 0: LOAD 0, 0 (s: P!GameState)
+	call stk := OpCode#Load(stk, s#8);
+	 // 1: GET (fieldname: STATE)
+	assert Seq#Length(stk) >= 1;
+	assert $Unbox(Seq#Index(stk, Seq#Length(stk)-1)) != null;
+	stk := Seq#Build(Seq#Take(stk, Seq#Length(stk)-1), $Box($srcHeap[$Unbox(Seq#Index(stk, Seq#Length(stk)-1)), FieldOfDecl(dtype($Unbox(Seq#Index(stk, Seq#Length(stk)-1))), _Field$STATE): Field (int)]));
+	 // 2: PUSH (intValue: 4)
+	call stk := OpCode#Pushi(stk, 4);
+	 // 3: INVOKE (argcount: 1) (opname: =~)
+	call stk := Native#OCLOperation#MatchingOperator
+		(stk, 
+		$Unbox(Seq#Index(stk,Seq#Length(stk)-1)): int,
+		$Unbox(Seq#Index(stk,Seq#Length(stk)-2)): int);
+	 // 4: IFN 10
+	b#4 := $Unbox(OpCode#Top(stk));
+	call stk := OpCode#Pop(stk);
+	if(!b#4){goto Label_10;}
+	 // 5: LOAD 0, 5 (act: P!Action)
+	call stk := OpCode#Load(stk, act#8);
+	 // 6: GET (fieldname: DONEBY)
+	assert Seq#Length(stk) >= 1;
+	assert $Unbox(Seq#Index(stk, Seq#Length(stk)-1)) != null;
+	stk := Seq#Build(Seq#Take(stk, Seq#Length(stk)-1), $Box($srcHeap[$Unbox(Seq#Index(stk, Seq#Length(stk)-1)), FieldOfDecl(dtype($Unbox(Seq#Index(stk, Seq#Length(stk)-1))), _Field$DONEBY): Field (int)]));
+	 // 7: PUSH (intValue: 2)
+	call stk := OpCode#Pushi(stk, 2);
+	 // 8: INVOKE (argcount: 1) (opname: =~)
+	call stk := Native#OCLOperation#MatchingOperator
+		(stk, 
+		$Unbox(Seq#Index(stk,Seq#Length(stk)-1)): int,
+		$Unbox(Seq#Index(stk,Seq#Length(stk)-2)): int);
+	 // 9: GOTO 11
+	goto Label_11;
+Label_10:
+	// 10: PUSHF
+	call stk := OpCode#Pushf(stk);
+Label_11:
+	// 11: IFN 18
+	b#11 := $Unbox(OpCode#Top(stk));
+	call stk := OpCode#Pop(stk);
+	if(!b#11){goto Label_18;}
+	// 12: LOAD 0, 5 (act: P!Action)
+	call stk := OpCode#Load(stk, act#8);
+	// 13: GET (fieldname: FRAME)
+	assert Seq#Length(stk) >= 1;
+	assert $Unbox(Seq#Index(stk, Seq#Length(stk)-1)) != null;
+	stk := Seq#Build(Seq#Take(stk, Seq#Length(stk)-1), $Box($srcHeap[$Unbox(Seq#Index(stk, Seq#Length(stk)-1)), FieldOfDecl(dtype($Unbox(Seq#Index(stk, Seq#Length(stk)-1))), _Field$FRAME): Field (int)]));
+	// 14: LOAD 0, 1 (rec: P!Record)
+	call stk := OpCode#Load(stk, rec#8);
+	// 15: GET (fieldname: FRAME)
+	assert Seq#Length(stk) >= 1;
+	assert $Unbox(Seq#Index(stk, Seq#Length(stk)-1)) != null;
+	stk := Seq#Build(Seq#Take(stk, Seq#Length(stk)-1), $Box($srcHeap[$Unbox(Seq#Index(stk, Seq#Length(stk)-1)), FieldOfDecl(dtype($Unbox(Seq#Index(stk, Seq#Length(stk)-1))), _Field$FRAME): Field (int)]));
+	// 16: INVOKE (argcount: 1) (opname: =~)
+	call stk := Native#OCLOperation#MatchingOperator
+		(stk, 
+		$Unbox(Seq#Index(stk,Seq#Length(stk)-1)): int,
+		$Unbox(Seq#Index(stk,Seq#Length(stk)-2)): int);
+	// 17: GOTO 19
+	goto Label_19;
+Label_18:
+	// 18: PUSHF
+	call stk := OpCode#Pushf(stk);
+Label_19:
+	// 19: IFN 25
+	b#19 := $Unbox(OpCode#Top(stk));
+	call stk := OpCode#Pop(stk);
+	if(!b#19){goto Label_25;}
+	// 20: LOAD 0, 5 (act: P!Action)
+	call stk := OpCode#Load(stk, act#8);
+	// 21: GET (fieldname: DIRECTION)
+	assert Seq#Length(stk) >= 1;
+	assert $Unbox(Seq#Index(stk, Seq#Length(stk)-1)) != null;
+	stk := Seq#Build(Seq#Take(stk, Seq#Length(stk)-1), $Box($srcHeap[$Unbox(Seq#Index(stk, Seq#Length(stk)-1)), FieldOfDecl(dtype($Unbox(Seq#Index(stk, Seq#Length(stk)-1))), _Field$DIRECTION): Field (int)]));
+	// 22: PUSH (intValue: 5)
+	call stk := OpCode#Pushi(stk, 5);
+	// 23: INVOKE (argcount: 1) (opname: =~)
+	call stk := Native#OCLOperation#MatchingOperator
+		(stk, 
+		$Unbox(Seq#Index(stk,Seq#Length(stk)-1)): int,
+		$Unbox(Seq#Index(stk,Seq#Length(stk)-2)): int);
+	// 24: GOTO 26
+	goto Label_26;
+Label_25:
+	// 25: PUSHF
+	call stk := OpCode#Pushf(stk);
+Label_26:
+	r:= $Unbox(OpCode#Top(stk));
+	call stk := OpCode#Pop(stk);
+}	 
